First sound semantic outcome triple

Outcome.v
@@ -8,59 +8,86 @@ Local Open Scope string_scope.
 Local Open Scope Z_scope.
 Local Open Scope list_scope.
 
-(* some old tactics *)
+Definition val := Z.
 
-(* Tactic Notation "inv" constr(h) := inversion h; subst. *)
-Tactic Notation "inj" constr(h) := injection h as h; subst.
-Tactic Notation "ok" := auto; try easy.
-
-(* these could be made less powerful in future, so they can't be used wrongly *)
-Tactic Notation "vacuous" := easy.
-(* Tactic Notation "ih" := ok. *)
-
-Tactic Notation "case_on" constr(e) := let H := fresh in destruct e eqn:H; ok.
-Tactic Notation "case_on" constr(e) ident(x) := destruct e eqn:x; ok.
-(* Tactic Notation "gen" ident_list(x) := generalize dependent x. *)
-
-(* new ones *)
-
-Ltac inv H := inversion H; clear H; subst.
-
-Module Flow3.
-
-  Definition val := Z.
-
-  Inductive expr : Type :=
-    | pvar (x: ident)
-    | pconst (n: val)
-    | plet (x: ident) (e1: expr) (e2: expr)
-    | passign (x1: ident) (x2: ident)
-    | pif (x: ident) (e1: expr) (e2: expr)
-    | pcall (x: ident) (a: ident)
-    .
-
-  Inductive eresult : Type :=
-    | enorm : val -> eresult
+Inductive expr : Type :=
+  | pvar (x: ident)
+  | pconst (n: val)
+  | plet (x: ident) (e1: expr) (e2: expr)
+  | passign (x1: ident) (x2: ident)
+  | pif (x: ident) (e1: expr) (e2: expr)
+  | pcall (x: ident) (a: ident)
   .
+
+(* Inductive eresult : Type :=
+  | enorm : val -> eresult
+  . *)
+Definition eresult := option val.
+
+Inductive fndef : Type := fn (i:ident) (b:expr).
+Definition fnenv : Type := ident -> option fndef.
+Definition fnenv_empty : fnenv := (fun _ => None).
+Definition fupdate (x: ident) (v: fndef) (s: fnenv) : fnenv :=
+  fun y => if string_dec x y then Some v else s y.
+
+Section Bigstep.
+
+  Variable fenv : fnenv.
 
   Reserved Notation " 'eval[' s ',' e ']' '=>' '[' s1 ',' r ']' " (at level 50, left associativity).
 
-  Inductive bigstep : store -> expr -> store -> eresult -> Prop :=
-    | eval_pvar : forall s x,
-      eval[ s, pvar x ]=>[ s, enorm (s x)]
+  CoInductive bigstep : store -> expr -> store -> eresult -> Prop :=
+
+    | eval_pvar : forall s x r,
+      s x = Some r ->
+      eval[ s, pvar x ]=>[ s, Some r ]
+
     | eval_pconst : forall s x,
-      eval[ s, pconst x ] => [ s, enorm x]
+      eval[ s, pconst x ] => [ s, Some x ]
+
     | eval_plet : forall x e1 e2 v s s2 s1 r,
-      eval[ s, e1 ] => [ s1, enorm v ] ->
+      eval[ s, e1 ] => [ s1, Some v ] ->
       eval[ supdate x v s1, e2 ] => [ s2, r] ->
       eval[ s, plet x e1 e2 ] => [ s, r ]
-    | eval_assign : forall x1 x2 s,
-      eval[ s, passign x1 x2 ] => [ s, enorm 0]
-      (* TODO call *)
-      (* TODO coinductive *)
 
-    where " 'eval[' s ',' e ']' '=>' '[' s1 ',' r ']' " := (bigstep s e s1 r)
+    | eval_pif_t : forall x e1 e2 s s1 r,
+      eval[ s, e1 ] => [ s1, r ] ->
+      s x = Some 0 ->
+      eval[ s, pif x e1 e2 ] => [ s1, r ]
+
+    | eval_pif_f : forall x e1 e2 s s1 r,
+      eval[ s, e2 ] => [ s1, r ] ->
+      s x <> Some 0 ->
+      eval[ s, pif x e1 e2 ] => [ s1, r ]
+
+    | eval_pcall : forall a f e s s1 r v y,
+      eval[ supdate y v s, e ] => [ s1, r ] ->
+      s a = Some v ->
+      fenv f = Some (fn y e) ->
+      eval[ s, pcall f a ] => [ s1, r ]
+
+    | eval_passign : forall x1 x2 s v s1,
+      s x2 = Some v ->
+      s1 = supdate x1 v s ->
+      eval[ s, passign x1 x2 ] => [ s1, Some 0 ]
+
+  where " 'eval[' s ',' e ']' '=>' '[' s1 ',' r ']' " := (bigstep s e s1 r)
   .
+
+  Example e1 : forall x1 x2 s,
+    s = supdate x2 1 (supdate x1 0 sempty) ->
+    eval[ s, passign x1 x2 ] =>
+      [ supdate x1 1 s, Some 0 ].
+  Proof.
+    intros.
+    apply eval_passign with (v := 1).
+    2: reflexivity.
+    rewrite H; now rewrite supdate_same.
+  Qed.
+
+  Inductive nati := n (n:nat) | inf.
+  Inductive resources := rb (l:nati) (u:nati).
+  Definition model := store -> resources -> Prop.
 
   Definition assertion := store -> Prop.
   Definition precond := assertion.
@@ -69,22 +96,116 @@ Module Flow3.
   Definition aand (P Q: assertion) : assertion :=
     fun s => P s /\ Q s.
 
+  Inductive rea := Term | MayLoop | Loop. (* resource assertion *)
+  Inductive lar := LR (d:precond) (r:rea). (* logic and resource *)
+
   Inductive outcome : Type :=
     | ok_er_nt : postcond -> precond -> precond -> outcome.
 
-  Inductive forward : precond -> expr -> outcome -> Prop :=
-    | f_pvar : forall x d,
-      forward d (pvar x) (ok_er_nt (fun r => aand d (fun s => r = s x)) d d)
-    | f_pconst : forall v d,
-      forward d (pconst v) (ok_er_nt (fun r => aand d (fun s => r = v)) d d)
-    (* | f_pconst : forall s x,
-      eval[ s, pconst x ] => [ s, enorm x]
-    | f_plet : forall x e1 e2 v s s2 s1 r,
-      eval[ s, e1 ] => [ s1, enorm v ] ->
-      eval[ supdate x v s1, e2 ] => [ s2, r] ->
-      eval[ s, plet x e1 e2 ] => [ s, r ]
-    | f_assign : forall x1 x2 s,
-      eval[ s, passign x1 x2 ] => [ s, enorm 0] *)
+  Definition ok_only (q:postcond) : outcome := ok_er_nt q (fun _ => False) (fun _ => False).
+
+  (* TODO sl entailment *)
+  (* TODO resource entailment *)
+  (* TODO case specs *)
+  (* TODO disjunction of D|R *)
+
+  (* TODO defn of compose is wrong *)
+
+  Definition compose (v:ident) (P Q:assertion) : assertion :=
+  (* say P is (fun s1 => s1 "x" = 1) *)
+    fun s => exists u, P (supdate v u s) /\ Q s
+    (* TODO this is existential on value, not variable *)
+    (* being able to refer to old(v) is a relational assertion *)
   .
 
-End Flow3.
+  CoInductive diverges : store -> expr -> Prop :=
+    | div_pcall : forall e y v s f a s1,
+      diverges s1 e ->
+      s1 = supdate y v s ->
+      fenv f = Some (fn y e) ->
+      diverges s (pcall f a)
+    .
+
+  Definition triple (P: precond) (e: expr) (Q: outcome) : Prop :=
+    forall ok er nt r s s1, Q = ok_er_nt ok er nt ->
+      P s ->
+          (eval[ s, e ] => [ s1, Some r ] -> ok r s1)
+        /\ (eval[ s, e ] => [ s1, None ] -> er s)
+        /\ (diverges s e -> nt s).
+
+  Lemma f_pconst : forall v p,
+    triple p (pconst v) (ok_only (fun r => aand p (fun s => r = v))).
+  Proof.
+    intros.
+    unfold triple.
+    intros.
+    unfold ok_only in H; injection H; clear H; intros.
+    repeat split; intros.
+    - inversion H3; subst; clear H3.
+      unfold aand; easy.
+    - inversion H3.
+    - inversion H3.
+  Qed.
+
+  Lemma f_passign : forall x1 x2 p,
+    triple p (passign x1 x2) (ok_only (fun _ => compose x1 p (fun s => s x1 = s x2))).
+  Proof.
+    intros.
+    unfold triple.
+    intros.
+    unfold ok_only in H; injection H; clear H; intros.
+    repeat split; intros.
+    - rewrite <- H2.
+      inversion H3; subst.
+      unfold compose.
+      exists v.
+      inversion H3; subst; clear H3.
+      split.
+      (* pose ident. *)
+      (* exists r. *)
+      admit.
+      rewrite H6.
+      f_equal.
+      admit.
+    - inversion H3.
+    - inversion H3.
+  Admitted.
+  (* Qed. *)
+
+  (* Inductive forward : precond -> expr -> outcome -> Prop :=
+
+    | f_pvar : forall x s,
+      forward s (pvar x) (ok_only (fun r => aand s (fun s => Some r = s x)))
+
+    | f_pconst : forall c s,
+      forward s (pconst c) (ok_only (fun r => aand s (fun s => r = c)))
+
+    | f_passign : forall x1 x2 s,
+      forward s (passign x1 x2) (ok_only (fun _ => compose x1 s (fun s => s x1 = s x2)))
+      (*
+        S o{v} (v=x)
+        ==> ex u. S[v:=u] /\ (v=x)[old(v):=u]
+        ==> ex u. S[v:=u] /\ v=x
+      *)
+. *)
+
+  (* Example e2 : forall x1 x2 s,
+    (* st = supdate x2 1 (supdate x1 0 sempty) -> *)
+    forward s (passign x1 x2) (ok_only (fun _ => fun s => s x1 = s x2)).
+  Proof.
+    intros.
+    constructor.
+  Qed. *)
+
+    (* TODO if *)
+    (* | f_pif : forall c s x e1 e2,
+      forward s (pif x e1 e2) (ok_only (fun r => aand s (fun s => r = c))) *)
+
+    (* TODO let *)
+
+    (* TODO call *)
+    (* | f_pcall : forall y b f c r x d,
+      fenv f = Some (fn y b) ->
+      forward (LR d r) (pcall f x) (ok_only (fun r => aand s (fun s => r = c))) *)
+  
+End Bigstep.
